Challenge/Modexp/Submission/Proofs/Fast/Paths/P2.lean
@@ -108,9 +108,9 @@ def blk1039 :
    pushAt 1131 1 1,
    pushAt 1132 2 4096,
    opAt 1133 .MSTORE,
-   pushAt 1134 2 4643,
+   pushAt 1134 2 3816,
    pushAt 1135 2 4096,
-   pushAt 1136 2 1911,
+   pushAt 1136 2 2534,
    opAt 1137 .JUMP]
 
 end Challenge.Modexp.Submission.Proofs.Fast
